Add heap implementation.

src/mem/Heaps.v
@@ -5,9 +5,61 @@ From Coq Require Import
   List
   Relations
   RelationClasses
-  Structures.Equalities.
+  Structures.Equalities
+  ZArith.
 
 Require Import Morphisms.
+
+From Coq Require Import
+  FSets.FMapAVL
+  FSets.FSetAVL.
+
+Import ListNotations.
+
+Module IM := FMapAVL.Make(Coq.Structures.OrderedTypeEx.Z_as_OT).
+Module IS := FSetAVL.Make(Coq.Structures.OrderedTypeEx.Z_as_OT).
+
+Lemma find_add_eq :
+  forall {elt} (m : @IM.t elt) (k : IM.key) (v : elt),
+    IM.find k (IM.add k v m) = Some v.
+Proof.
+  intros elt m k v.
+  apply IM.find_1.
+  apply IM.add_1; auto.
+Qed.
+
+Lemma find_add_neq :
+  forall {elt} (m : @IM.t elt) (k1 k2 : IM.key) (v x : elt),
+    k1 <> k2 ->
+    IM.find k1 m = Some x ->
+    IM.find k1 (IM.add k2 v m) = Some x.
+Proof.
+  intros elt m k1 k2 v x NEQ FIND.
+  apply IM.find_1.
+  apply IM.add_2; auto.
+  apply IM.find_2; auto.
+Qed.
+
+Lemma IS_mem_add_eq :
+  forall (m : IS.t) (k : IS.elt),
+    IS.mem k (IS.add k m) = true.
+Proof.
+  intros m k.
+  apply IS.mem_1.
+  apply IS.add_1; auto.
+Qed.
+
+Lemma IS_mem_add_neq :
+  forall (m : IS.t) (k1 k2 : IS.elt),
+    k1 <> k2 ->
+    IS.mem k1 m = true ->
+    IS.mem k1 (IS.add k2 m) = true.
+Proof.
+  intros m k1 k2 NEQ IN.
+  apply IS.mem_1.
+  apply IS.add_2; auto.
+  apply IS.mem_2; auto.
+Qed.
 
 Module Type CORE_HEAP
   (Import ADDR : BASIC_ADDRESS) <: Typ.
@@ -21,7 +73,7 @@ Module Type CORE_HEAP
 
   (** Is a pointer allocated in the heap under a root pointer *)
   Parameter ptr_in_heap : t -> addr -> addr -> bool.
-  Parameter ptrs_in_heap : t -> addr -> list addr.
+  Parameter ptrs_in_heap : t -> addr -> list Z.
 
   (** Add a pointer to the heap under a root pointer *)
   Parameter add_ptr_to_heap : t -> addr -> addr -> t.
@@ -65,7 +117,7 @@ Module Type CORE_HEAP
 
   Parameter ptr_in_heap_ptrs_in_heap :
     forall h root ptr,
-      ptr_in_heap h root ptr = true <-> In ptr (ptrs_in_heap h root).
+      ptr_in_heap h root ptr = true <-> In (ptr_to_int ptr) (ptrs_in_heap h root).
 
   Parameter free_root_in_heap_root_not_in_heap :
     forall h root,
@@ -75,7 +127,7 @@ Module Type CORE_HEAP
   Parameter free_root_in_heap_removes_root :
     forall h root h',
       free_root_in_heap h root = Some h' ->
-      root_ptr_in_heap h root = false.
+      root_ptr_in_heap h' root = false.
 
   Parameter free_root_in_heap_removes_ptrs :
     forall h root h',
@@ -160,3 +212,269 @@ Module Type HEAP_EXTRAS
 End HEAP_EXTRAS.
 
 Module Type HEAP (ADDR : BASIC_ADDRESS) := CORE_HEAP ADDR <+ HEAP_NOTATIONS ADDR <+ HEAP_EQV ADDR <+ HEAP_EXTRAS ADDR.
+
+
+(*** IntMap based heap implementation *)
+Module CORE_HEAP_INTMAP (Import ADDR : BASIC_ADDRESS) <: CORE_HEAP ADDR.
+  Definition Block := IS.t.
+
+  Definition t := IM.t Block.
+  Definition empty_heap : t := @IM.empty Block.
+
+  (*** Heap operations *)
+
+  (** Is a pointer a root pointer of the heap *)
+  Definition root_ptr_in_heap (h : t) (ptr : addr) : bool :=
+    IM.mem (ptr_to_int ptr) h.
+
+  (** Is a pointer allocated in the heap under a root pointer *)
+  Definition ptr_in_heap (h : t) (root ptr : addr) : bool :=
+    match IM.find (ptr_to_int root) h with
+    | None => false
+    | Some ptrs =>
+        IS.mem (ptr_to_int ptr) ptrs
+    end.
+
+  Definition ptrs_in_heap (h : t) (root : addr) : list Z :=
+    match IM.find (ptr_to_int root) h with
+    | None => nil
+    | Some ptrs => IS.elements ptrs
+    end.
+
+  (** Add a pointer to the heap under a root pointer *)
+  Definition add_ptr_to_heap (h : t) (root ptr : addr) : t :=
+    if ptr_in_heap h root ptr
+    then h
+    else
+      match IM.find (ptr_to_int root) h with
+      | None =>
+          IM.add (ptr_to_int root) (IS.singleton (ptr_to_int ptr)) h
+      | Some ptrs =>
+          IM.add (ptr_to_int root) (IS.add (ptr_to_int ptr) ptrs) h
+      end.
+
+  (** Free a root pointer *)
+  Definition free_root_in_heap (h : t) (root : addr) : option t :=
+    if root_ptr_in_heap h root
+    then Some (IM.remove (ptr_to_int root) h)
+    else None.
+
+  (*** Heap properties *)
+
+  Lemma empty_heap_ptr_spec :
+    forall root ptr,
+      ptr_in_heap empty_heap root ptr = false.
+  Proof.
+    intros root ptr; cbn; auto.
+  Qed.
+
+  Lemma empty_heap_root_spec :
+    forall ptr,
+      root_ptr_in_heap empty_heap ptr = false.
+  Proof.
+    intros ptr; cbn; auto.
+  Qed.
+
+  Lemma add_ptr_to_heap_ptr_in_heap_new :
+    forall h root ptr,
+      ptr_in_heap (add_ptr_to_heap h root ptr) root ptr = true.
+  Proof.
+    intros h root ptr.
+    unfold add_ptr_to_heap.
+    destruct (ptr_in_heap h root ptr) eqn:PTR; auto.
+    unfold ptr_in_heap.
+    destruct (IM.find (ptr_to_int root) h) eqn:FIND;
+      rewrite find_add_eq.
+    - apply IS_mem_add_eq.
+    - apply IS.mem_1. apply IS.singleton_2; auto.
+  Qed.
+
+  (* May not hold for `ptr_in_heap h ptr = false`, because we may
+     consider different pointers with the same provenance to be in a
+     heap if they share a physical address *)
+  Lemma add_ptr_to_heap_ptr_in_heap_old :
+    forall h root ptr root_old ptr_old,
+      ptr_in_heap h root_old ptr_old = true ->
+      ptr_in_heap (add_ptr_to_heap h root ptr) root_old ptr_old = true.
+  Proof.
+    intros h root ptr root_old ptr_old IN.
+    destruct (BinInt.Z.eq_dec (ptr_to_int root) (ptr_to_int root_old)) as [EQROOT | NEQROOT].
+    {
+      unfold add_ptr_to_heap.
+      destruct (ptr_in_heap h root ptr) eqn:PTR; auto.
+      unfold ptr_in_heap in *.
+      rewrite EQROOT in PTR.
+      rewrite EQROOT.
+      destruct (IM.find (elt:=Block) (ptr_to_int root_old) h) eqn:FIND; try discriminate.
+
+      rewrite find_add_eq.
+      apply IS_mem_add_neq; auto.
+      { intros CONTRA.
+        rewrite CONTRA in IN.
+        rewrite PTR in IN; discriminate.
+      }
+    }
+
+    {
+      unfold add_ptr_to_heap.
+      destruct (ptr_in_heap h root ptr) eqn:PTR; auto.
+      unfold ptr_in_heap in *.
+      destruct (IM.find (elt:=Block) (ptr_to_int root_old) h) eqn:FIND_OLD; try discriminate.
+      apply IM.find_2 in FIND_OLD.
+      destruct (IM.find (ptr_to_int root) h) eqn:FIND;
+        erewrite find_add_neq; eauto;
+        apply IM.find_1; auto.
+    }
+  Qed.
+
+  Lemma add_ptr_to_heap_root_ptr_in_heap_new :
+    forall h root ptr,
+      root_ptr_in_heap (add_ptr_to_heap h root ptr) root = true.
+  Proof.
+    intros h root ptr.
+    unfold add_ptr_to_heap.
+    destruct (ptr_in_heap h root ptr) eqn:PTR; auto.
+    - unfold root_ptr_in_heap.
+      unfold ptr_in_heap in *.
+      destruct (IM.find (elt:=Block) (ptr_to_int root) h) eqn:FIND; try discriminate.
+      apply IM.mem_1.
+      exists b.
+      apply IM.find_2; auto.
+    - unfold root_ptr_in_heap.
+      unfold ptr_in_heap in *.
+      destruct (IM.find (elt:=Block) (ptr_to_int root) h) eqn:FIND; try discriminate;
+        apply IM.mem_1;
+        eexists; apply IM.add_1; eauto.
+  Qed.
+
+  (* May not hold for `root_ptr_in_heap h root = false`, because we may
+     consider different pointers with the same provenance to be in a
+     heap if they share a physical address *)
+  Lemma add_ptr_to_heap_root_ptr_in_heap_old :
+    forall h root ptr root_old,
+      root_ptr_in_heap h root_old = true ->
+      root_ptr_in_heap (add_ptr_to_heap h root ptr) root_old = true.
+  Proof.
+    intros h root ptr root_old ROOT.
+    unfold add_ptr_to_heap.
+    unfold root_ptr_in_heap in *.
+    unfold ptr_in_heap in *.
+    destruct (BinInt.Z.eq_dec (ptr_to_int root) (ptr_to_int root_old)) as [EQ | NEQ].
+    - destruct (IM.find (elt:=Block) (ptr_to_int root) h) eqn:FIND.
+      + destruct (IS.mem (ptr_to_int ptr) b) eqn:EX; auto.
+        apply IM.mem_1.
+        eexists; apply IM.add_1; auto.
+      + apply IM.mem_1.
+        eexists; apply IM.add_1; auto.
+    - destruct (IM.find (elt:=Block) (ptr_to_int root) h) eqn:FIND.
+      + destruct (IS.mem (ptr_to_int ptr) b) eqn:EX; auto.
+        apply IM.mem_1.
+        apply IM.mem_2 in ROOT as (x & ROOT).
+        eexists; apply IM.add_2; eauto.
+      + apply IM.mem_1.
+        apply IM.mem_2 in ROOT as (x & ROOT).
+        eexists; apply IM.add_2; eauto.
+  Qed.
+
+  Lemma ptr_in_heap_ptrs_in_heap :
+    forall h root ptr,
+      ptr_in_heap h root ptr = true <-> In (ptr_to_int ptr) (ptrs_in_heap h root).
+  Proof.
+    intros h root ptr.
+    unfold ptr_in_heap, ptrs_in_heap.
+    split; intros IN.
+    - destruct (IM.find (elt:=Block) (ptr_to_int root) h) eqn:FIND; try discriminate.
+      apply IS.mem_2 in IN.
+      apply IS.elements_1 in IN.
+      apply SetoidList.InA_alt in IN as (y&EQV&IN); subst; auto.
+    - destruct (IM.find (elt:=Block) (ptr_to_int root) h) eqn:FIND.
+      + apply IS.mem_1.
+        apply IS.elements_2.
+        apply SetoidList.InA_alt.
+        eexists; split; eauto.
+      + inversion IN.
+  Qed.
+
+  Lemma free_root_in_heap_root_not_in_heap :
+    forall h root,
+      root_ptr_in_heap h root = false ->
+      free_root_in_heap h root = None.
+  Proof.
+    intros h root ROOT.
+    unfold free_root_in_heap.
+    rewrite ROOT.
+    auto.
+  Qed.
+
+  Lemma free_root_in_heap_removes_root :
+    forall h root h',
+      free_root_in_heap h root = Some h' ->
+      root_ptr_in_heap h' root = false.
+  Proof.
+    intros h root h' FREE.
+    unfold free_root_in_heap in *.
+    unfold root_ptr_in_heap in *.
+    destruct (IM.mem (elt:=Block) (ptr_to_int root) h) eqn:MEM; try discriminate.
+    inversion FREE.
+    destruct (IM.mem (elt:=Block) (ptr_to_int root) (IM.remove (elt:=Block) (ptr_to_int root) h)) eqn:REM; auto.
+    apply IM.mem_2 in REM.
+    exfalso.
+    eapply IM.remove_1; [|apply REM]; auto.
+  Qed.
+
+  Lemma free_root_in_heap_removes_ptrs :
+    forall h root h',
+      free_root_in_heap h root = Some h' ->
+      forall ptr, ptr_in_heap h root ptr = true -> ptr_in_heap h' root ptr = false.
+  Proof.
+    intros h root h' FREE ptr IN.
+    unfold free_root_in_heap in *.
+    unfold root_ptr_in_heap in *.
+    unfold ptr_in_heap in *.
+    destruct (IM.find (elt:=Block) (ptr_to_int root) h) eqn:FIND; try discriminate.
+    assert (IM.mem (elt:=Block) (ptr_to_int root) h = true) as ROOT_IN.
+    { apply IM.mem_1.
+      exists b. apply IM.find_2; eauto.
+    }
+
+    rewrite ROOT_IN in FREE.
+    inversion FREE.
+
+    destruct (IM.find (elt:=Block) (ptr_to_int root) (IM.remove (elt:=Block) (ptr_to_int root) h)) eqn:REM; auto.
+    exfalso.
+
+    eapply IM.remove_1; cycle 1.
+    exists b0. apply IM.find_2; eauto.
+    auto.
+  Qed.
+
+  Lemma free_root_in_heap_preserves_other_roots :
+    forall h root root' h',
+      ptr_to_int root <> ptr_to_int root' ->
+      free_root_in_heap h root = Some h' ->
+      forall ptr, ptr_in_heap h root' ptr = ptr_in_heap h' root' ptr.
+  Proof.
+    intros h root root' h' NEQ FREE ptr.
+    unfold free_root_in_heap in *.
+    unfold root_ptr_in_heap in *.
+    unfold ptr_in_heap in *.
+
+    destruct (IM.mem (elt:=Block) (ptr_to_int root) h) eqn:MEM; try discriminate.
+    inversion FREE; subst.
+
+    destruct (IM.find (elt:=Block) (ptr_to_int root') (IM.remove (elt:=Block) (ptr_to_int root) h)) eqn:REM.
+    + erewrite IM.find_1; try reflexivity.
+      eapply IM.remove_3; apply IM.find_2; eauto.
+    + destruct (IM.find (elt:=Block) (ptr_to_int root') h) eqn:FIND; auto.
+      exfalso.
+      replace (IM.find (elt:=Block) (ptr_to_int root') (IM.remove (elt:=Block) (ptr_to_int root) h)) with (Some b) in REM; cycle 1.
+
+      symmetry.
+      apply IM.find_1. apply IM.remove_2; auto.
+      apply IM.find_2; auto.
+
+      discriminate.
+  Qed.
+End CORE_HEAP_INTMAP.
+
+Module HEAP_IMPL (ADDR : BASIC_ADDRESS) <: HEAP ADDR := CORE_HEAP_INTMAP ADDR <+ HEAP_NOTATIONS ADDR <+ HEAP_EQV ADDR <+ HEAP_EXTRAS ADDR.
